\label{sec:annex_shape_functions}
\subsection{Lineare Dreieckselemente}
\label{sec:linear_triangles_annex}

\begin{minipage}[t]{0.3\textwidth}
\subsubsection{Formfunktionen}
\begin{align*}
	&N_1 = 1 - \xi - \eta\\
	&N_2 = \xi \\
	&N_3 = \eta
\end{align*}
\end{minipage}
\begin{minipage}[t]{0.3\textwidth}
\subsubsection{Partielle Ableitungen nach $\xi$}
\begin{align*}
&\parDiff{N1}{\xi} = -1\\
&\parDiff{N_2}{\xi} = 1\\
&\parDiff{N_3}{\xi} = 0
\end{align*}
\end{minipage}
\begin{minipage}[t]{0.3\textwidth}
\subsubsection{Partielle Ableitungen nach $\eta$}
\begin{align*}
&\parDiff{N_1}{\eta} = -1\\
&\parDiff{N_2}{\eta} = 0\\
&\parDiff{N_3}{\eta} = 1
\end{align*}
\end{minipage}



\subsection{Quadratische Dreieckselemente}
\label{sec:quadratic_triangles_annex}
\begin{minipage}[t]{0.3\textwidth}
\subsubsection{Formfunktionen}
\begin{align*}
&N_1 = (1 - \xi - \eta)(1 - 2\xi - 2\eta)\\
&N_2 = 4\xi (1 - \xi - \eta) \\
&N_3 = \xi (2 \xi - 1)\\
&N_4 = 4 \xi \eta \\
&N_5 = \eta (2\eta - 1)\\
&N_6 = -4\eta (1 - \xi - \eta)
\end{align*}
\end{minipage}
\begin{minipage}[t]{0.3\textwidth}
\subsubsection{Partielle Ableitungen nach $\xi$}
\begin{align*}
&\parDiff{N_1}{\xi} = -3 + 4\xi + 4\eta\\
&\parDiff{N_2}{\xi} = 4 - 8\xi - 4\eta\\
&\parDiff{N_3}{\xi} = 4\xi - 1\\
&\parDiff{N_4}{\xi} = 4\eta\\
&\parDiff{N_5}{\xi} = 0\\
&\parDiff{N_6}{\xi} = -4\eta\\
\end{align*}
\end{minipage}
\begin{minipage}[t]{0.3\textwidth}
\subsubsection{Partielle Ableitungen nach $\eta$}
\begin{align*}
&\parDiff{N_1}{\eta} = -3 + 4\xi + 4\eta\\
&\parDiff{N_2}{\eta} = -4\xi \\
&\parDiff{N_3}{\eta} = 0\\
&\parDiff{N_4}{\eta} = 4\xi\\
&\parDiff{N_5}{\eta} = 4\eta - 1\\
&\parDiff{N_6}{\eta} = 4 - 4\xi - 8\eta\\
\end{align*}
\end{minipage}

\subsection{Kubische Dreieckselemente}
\label{sec:cubic_triangles_annex}
\subsubsection{Formfunktionen}

\begin{align*}
&N_1 = -\frac{9\eta ^3}{2}-\frac{27\eta ^2\xi}{2}+9\eta ^2-\frac{27\eta {\xi}^2}{2}+18\eta \xi-\frac{11\eta }{2}-\frac{9{\xi}^3}{2}+9{\xi}^2-\frac{11\xi}{2}+1\\
&N_2 = \frac{27\eta ^2\xi}{2}+27\eta {\xi}^2-\frac{45\eta \xi}{2}+\frac{27{\xi}^3}{2}-\frac{45{\xi}^2}{2}+9\xi \\
&N_3 = \frac{9\eta \xi}{2}-\frac{9\xi}{2}-\frac{27\eta {\xi}^2}{2}+18{\xi}^2-\frac{27{\xi}^3}{2}\\
&N_4 = \frac{9{\xi}^3}{2}-\frac{9{\xi}^2}{2}+\xi \\
&N_5 = \frac{27\eta {\xi}^2}{2}-\frac{9\eta \xi}{2}\\
&N_6 = \frac{27\eta ^2\xi}{2}-\frac{9\eta \xi}{2}\\
&N_7 = \frac{9\eta ^3}{2}-\frac{9\eta ^2}{2}+\eta \\
&N_8 = \frac{9\eta \xi}{2}-\frac{9\eta }{2}-\frac{27\eta ^2\xi}{2}+18\eta ^2-\frac{27\eta ^3}{2}\\
&N_9 = \frac{27\eta ^3}{2}+27\eta ^2\xi-\frac{45\eta ^2}{2}+\frac{27\eta {\xi}^2}{2}-\frac{45\eta \xi}{2}+9\eta \\
&N_{10} = -27\eta ^2\xi-27\eta {\xi}^2+27\eta \xi
\end{align*}

\begin{minipage}[t]{0.45\textwidth}

\subsubsection{Partielle Ableitungen nach $\xi$}
\begin{align*}
&\parDiff{N_1}{\xi} = -\frac{27\eta ^2}{2}-27\eta \zeta+18\eta -\frac{27{\zeta}^2}{2}+18\zeta-\frac{11}{2}\\
&\parDiff{N_2}{\xi} = \frac{27\eta ^2}{2}+54\eta \zeta-\frac{45\eta }{2}+\frac{81{\zeta}^2}{2}-45\zeta+9\\
&\parDiff{N_3}{\xi} = \frac{9\eta }{2}+36\zeta-27\eta \zeta-\frac{81{\zeta}^2}{2}-\frac{9}{2}\\
&\parDiff{N_4}{\xi} = \frac{27{\zeta}^2}{2}-9\zeta+1\\
&\parDiff{N_5}{\xi} = 27\eta \zeta-\frac{9\eta }{2}\\
&\parDiff{N_6}{\xi} = \frac{27\eta ^2}{2}-\frac{9\eta }{2}\\
&\parDiff{N_7}{\xi} = 0\\
&\parDiff{N_8}{\xi} = \frac{9\eta }{2}-\frac{27\eta ^2}{2}\\
&\parDiff{N_9}{\xi} = 27\eta \zeta-\frac{45\eta }{2}+27\eta ^2\\
&\parDiff{N_{10}}{\xi} = 27\eta -54\eta \zeta-27\eta ^2\\
\end{align*}
\end{minipage}
\hspace{5mm}
\begin{minipage}[t]{0.45\textwidth}
\subsubsection{Partielle Ableitungen nach $\eta$}
\begin{align*}
&\parDiff{N_1}{\eta} = -\frac{27\eta ^2}{2}-27\eta \zeta+18\eta -\frac{27{\zeta}^2}{2}+18\zeta-\frac{11}{2}\\
&\parDiff{N_2}{\eta} = 27\eta \zeta-\frac{45\zeta}{2}+27{\zeta}^2\\
&\parDiff{N_3}{\eta} = \frac{9\zeta}{2}-\frac{27{\zeta}^2}{2}\\
&\parDiff{N_4}{\eta} = 0\\
&\parDiff{N_5}{\eta} = \frac{27{\zeta}^2}{2}-\frac{9\zeta}{2}\\
&\parDiff{N_6}{\eta} = 27\eta \zeta-\frac{9\zeta}{2}\\
&\parDiff{N_7}{\eta} = \frac{27\eta ^2}{2}-9\eta +1\\
&\parDiff{N_8}{\eta} = 36\eta +\frac{9\zeta}{2}-27\eta \zeta-\frac{81\eta ^2}{2}-\frac{9}{2}\\
&\parDiff{N_9}{\eta} = \frac{81\eta ^2}{2}+54\eta \zeta-45\eta +\frac{27{\zeta}^2}{2}-\frac{45\zeta}{2}+9\\
&\parDiff{N_{10}}{\eta} = 27\zeta-54\eta \zeta-27{\zeta}^2\\
\end{align*}
\end{minipage}